disk-betree/BlockCache.dfy
@@ -156,9 +156,9 @@ abstract module BlockCache refines Transactable {
     && BlockPointsToValidReferences(block, s.ephemeralSuperblock.refcounts)
   }
 
-  predicate Reads(k: Constants, s: Variables, ref: Reference, block: Node)
+  predicate ReadStep(k: Constants, s: Variables, op: ReadOp)
   {
-    s.Ready? && MapsTo(s.cache, ref, block)
+    s.Ready? && MapsTo(s.cache, op.ref, op.block)
   }
 
   predicate OpStep(k: Constants, s: Variables, s': Variables, op: Op)
